mm0-lean/x86/determ.lean
@@ -1,51 +1,55 @@
 import x86.x86 data.list.basic
 
-namespace x86
+namespace bitvec
 
-def decoder := state_t (list byte) option
-instance : monad decoder := state_t.monad
 
-def read1 : decoder byte :=
-⟨λ l, list.cases_on l none (λ b l, some (b, l))⟩
+@[class] def reify {n} (v : bitvec n) (l : out_param (list bool)) : Prop :=
+from_bits_fill ff l = v
 
-@[class] def bitvec.reify {n} (v : bitvec n) (l : out_param (list bool)) : Prop :=
-bitvec.from_bits_fill ff l = v
+theorem reify.mk {n} (v) {l} [h : @reify n v l] :
+  from_bits_fill ff l = v := h
 
-theorem bitvec.reify.mk {n} (v) {l} [h : @bitvec.reify n v l] :
-  bitvec.from_bits_fill ff l = v := h
+theorem reify_eq {n v l l'} [@reify n v l] (h : l' = v.1) :
+  l' = (@from_bits_fill ff l n).1 := by rwa reify.mk v
+theorem reify_eq' {n v l l'} [@reify n v l] (h : l' = v) :
+  l' = @from_bits_fill ff l n := by rwa reify.mk v
 
-theorem bitvec.reify_eq {n v l l'} [@bitvec.reify n v l] (h : l' = v.1) :
-  l' = (@bitvec.from_bits_fill ff l n).1 := by rwa bitvec.reify.mk v
-theorem bitvec.reify_eq' {n v l l'} [@bitvec.reify n v l] (h : l' = v) :
-  l' = @bitvec.from_bits_fill ff l n := by rwa bitvec.reify.mk v
+theorem from_bits_fill_eq : ∀ {n b l} (e : list.length l = n),
+  from_bits_fill b l = ⟨l, e⟩
+| 0     b []       e := rfl
+| (n+1) b (a :: l) e :=
+  by rw [from_bits_fill, from_bits_fill_eq (nat.succ_inj e)]; refl
 
-theorem bitvec.bits_to_nat_zero (n) : bitvec.bits_to_nat (list.repeat ff n) = 0 :=
-by simp [bitvec.bits_to_nat]; induction n; simp *
+theorem bits_to_nat_zero (n) : bits_to_nat (list.repeat ff n) = 0 :=
+by simp [bits_to_nat]; induction n; simp *
 
-@[simp] theorem bitvec.to_nat_nil : bitvec.to_nat vector.nil = 0 := rfl
+@[simp] theorem bits_to_nat_cons (a l) :
+  bits_to_nat (a :: l) = nat.bit a (bits_to_nat l) := rfl
 
-@[simp] theorem bitvec.to_nat_zero (n) : bitvec.to_nat (0 : bitvec n) = 0 :=
-bitvec.bits_to_nat_zero _
+@[simp] theorem to_nat_nil : to_nat vector.nil = 0 := rfl
 
-@[simp] theorem bitvec.to_nat_cons (b) {n} (v : bitvec n) :
-  bitvec.to_nat (b :: v) = nat.bit b (bitvec.to_nat v) := 
+@[simp] theorem to_nat_zero (n) : to_nat (0 : bitvec n) = 0 :=
+bits_to_nat_zero _
+
+@[simp] theorem to_nat_cons (b) {n} (v : bitvec n) :
+  to_nat (b :: v) = nat.bit b (to_nat v) :=
 by cases v; refl
 
-@[simp] theorem bitvec.of_nat_succ (n i : ℕ) :
+@[simp] theorem of_nat_succ (n i : ℕ) :
   bitvec.of_nat n.succ i = i.bodd :: bitvec.of_nat n i.div2 :=
 by rw [bitvec.of_nat, nat.bodd_div2_eq, bitvec.of_nat]
 
-@[simp] theorem bitvec.of_nat_bit (n : ℕ) (b i) :
+@[simp] theorem of_nat_bit (n : ℕ) (b i) :
   bitvec.of_nat n.succ (nat.bit b i) = b :: bitvec.of_nat n i :=
-by rw [bitvec.of_nat_succ, nat.div2_bit, nat.bodd_bit]
+by rw [of_nat_succ, nat.div2_bit, nat.bodd_bit]
 
-theorem bitvec.of_nat_zero (n) : bitvec.of_nat n 0 = 0 :=
+theorem of_nat_zero (n) : bitvec.of_nat n 0 = 0 :=
 by induction n; [refl, exact congr_arg (vector.cons ff) n_ih]
 
-theorem bitvec.of_nat_one (n) : bitvec.of_nat n 1 = 1 :=
-by cases n; [refl, exact congr_arg (vector.cons tt) (bitvec.of_nat_zero _)]
+theorem of_nat_one (n) : bitvec.of_nat n 1 = 1 :=
+by cases n; [refl, exact congr_arg (vector.cons tt) (of_nat_zero _)]
 
-theorem bitvec.to_nat_nth {n} (i j) :
+theorem to_nat_nth {n} (i j) :
   (bitvec.of_nat n i).nth j = i.test_bit j.1 :=
 begin
   generalize e : bitvec.of_nat n i = v, cases v with l e',
@@ -61,93 +65,117 @@ begin
   exact n_ih _ _ _ _ e₂ (nat.lt_of_succ_lt_succ h)
 end
 
-theorem bitvec.of_nat_bits_to_nat {n} (l : list bool) :
-  bitvec.of_nat n (bitvec.bits_to_nat l) = bitvec.from_bits_fill ff l :=
+theorem of_nat_bits_to_nat {n} (l : list bool) :
+  bitvec.of_nat n (bits_to_nat l) = from_bits_fill ff l :=
 begin
-  rw bitvec.bits_to_nat,
-  induction l generalizing n, exact bitvec.of_nat_zero _,
+  rw bits_to_nat,
+  induction l generalizing n, exact of_nat_zero _,
   cases n, refl,
-  simp [*, bitvec.bits_to_nat, bitvec.from_bits_fill,
+  simp [*, bits_to_nat, from_bits_fill,
     bitvec.of_nat, nat.bodd_bit, nat.div2_bit]
 end
 
-theorem bitvec.reify_iff {n v l} : @bitvec.reify n v l ↔ bitvec.of_nat n (bitvec.bits_to_nat l) = v :=
-iff_of_eq $ congr_arg (= v) (bitvec.of_nat_bits_to_nat _).symm
+theorem reify_iff {n v l} : @reify n v l ↔ bitvec.of_nat n (bits_to_nat l) = v :=
+iff_of_eq $ congr_arg (= v) (of_nat_bits_to_nat _).symm
 
-theorem bitvec.of_nat_bits_to_nat_eq {n} (l : list bool) (e : l.length = n) :
-  bitvec.of_nat n (bitvec.bits_to_nat l) = ⟨l, e⟩ :=
+theorem of_nat_bits_to_nat_eq {n} (l : list bool) (e : l.length = n) :
+  bitvec.of_nat n (bits_to_nat l) = ⟨l, e⟩ :=
 begin
   induction n generalizing l; cases l; injection e, refl,
-  simp [bitvec.bits_to_nat, nat.div2_bit, nat.bodd_bit],
+  simp [bits_to_nat, nat.div2_bit, nat.bodd_bit],
   exact congr_arg (vector.cons l_hd) (n_ih _ h_1)
 end
 
-theorem bitvec.of_nat_to_nat : ∀ {n} (v : bitvec n),
-  bitvec.of_nat n (bitvec.to_nat v) = v
-| n ⟨l, e⟩ := bitvec.of_nat_bits_to_nat_eq l e
+theorem of_nat_to_nat : ∀ {n} (v : bitvec n),
+  bitvec.of_nat n (to_nat v) = v
+| n ⟨l, e⟩ := of_nat_bits_to_nat_eq l e
 
-theorem bitvec.of_nat_from_bits_fill (n m i) (h : n ≤ m) :
-  bitvec.of_nat n i = bitvec.from_bits_fill ff (bitvec.of_nat m i).1 :=
+theorem of_nat_from_bits_fill (n m i) (h : n ≤ m) :
+  bitvec.of_nat n i = from_bits_fill ff (bitvec.of_nat m i).1 :=
 begin
   generalize e : bitvec.of_nat m i = v, cases v with l h, simp,
   induction n generalizing m i l e, exact (vector.eq_nil _).trans (vector.eq_nil _).symm,
-  rw [bitvec.of_nat_succ], 
+  rw [of_nat_succ],
   cases m, cases h,
-  rw [bitvec.of_nat_succ] at e,
+  rw [of_nat_succ] at e,
   generalize e' : bitvec.of_nat m i.div2 = v, cases v with l' h',
   rw e' at e, injection e, subst l,
-  rw [n_ih _ _ (nat.le_of_succ_le_succ h) _ _ e', bitvec.from_bits_fill],
+  rw [n_ih _ _ (nat.le_of_succ_le_succ h) _ _ e', from_bits_fill],
 end
 
-theorem bitvec.of_nat_bit0_aux {n} (j : bitvec (nat.succ n)) :
-  bit0 j = ff :: bitvec.from_bits_fill ff (j.val) := 
+theorem of_nat_bit0_aux {n} (j : bitvec (nat.succ n)) :
+  bit0 j = ff :: from_bits_fill ff (j.val) :=
 begin
-  change bitvec.of_nat n.succ (bit0 (bitvec.to_nat j)) = _,
-  rw [bitvec.of_nat_succ,
-    nat.bodd_bit0, nat.div2_bit0, bitvec.to_nat, bitvec.of_nat_bits_to_nat]
+  change bitvec.of_nat n.succ (bit0 (to_nat j)) = _,
+  rw [of_nat_succ,
+    nat.bodd_bit0, nat.div2_bit0, to_nat, of_nat_bits_to_nat]
 end
 
-theorem bitvec.of_nat_bit0 (n i) : bitvec.of_nat n (bit0 i) = bit0 (bitvec.of_nat n i) :=
+theorem of_nat_bit0 (n i) : bitvec.of_nat n (bit0 i) = bit0 (bitvec.of_nat n i) :=
 begin
   induction n generalizing i, refl,
-  rw [bitvec.of_nat_succ,
+  rw [of_nat_succ,
     nat.bodd_bit0, nat.div2_bit0],
-  rw [bitvec.of_nat_from_bits_fill _ _ _ (nat.le_succ _)],
+  rw [of_nat_from_bits_fill _ _ _ (nat.le_succ _)],
   generalize : bitvec.of_nat n_n.succ i = j,
-  rw bitvec.of_nat_bit0_aux,
+  rw of_nat_bit0_aux,
 end
 
-theorem bitvec.of_nat_bit1 (n i) : bitvec.of_nat n (bit1 i) = bit1 (bitvec.of_nat n i) :=
+theorem of_nat_bit1 (n i) : bitvec.of_nat n (bit1 i) = bit1 (bitvec.of_nat n i) :=
 begin
   induction n generalizing i, refl,
-  rw [bitvec.of_nat_succ,
+  rw [of_nat_succ,
     nat.bodd_bit1, nat.div2_bit1],
-  rw [bitvec.of_nat_from_bits_fill _ _ _ (nat.le_succ _)],
+  rw [of_nat_from_bits_fill _ _ _ (nat.le_succ _)],
   generalize : bitvec.of_nat n_n.succ i = j,
-  change _ = bitvec.of_nat _ (bitvec.to_nat (bit0 j) + bit0 (@bitvec.to_nat n_n 0) + 1),
-  rw [bitvec.to_nat_zero],
-  change _ = bitvec.of_nat _ (bitvec.to_nat (bit0 j) + 1),
-  rw [bitvec.of_nat_bit0_aux, bitvec.to_nat_cons],
+  change _ = bitvec.of_nat _ (to_nat (bit0 j) + bit0 (@to_nat n_n 0) + 1),
+  rw [to_nat_zero],
+  change _ = bitvec.of_nat _ (to_nat (bit0 j) + 1),
+  rw [of_nat_bit0_aux, to_nat_cons],
   change _ = bitvec.of_nat _ (nat.bit tt _),
-  rw [bitvec.of_nat_bit, bitvec.of_nat_to_nat],
+  rw [of_nat_bit, of_nat_to_nat],
 end
 
-instance bitvec.reify_0 {n} : @bitvec.reify n 0 [] := rfl
+instance reify_0 {n} : @reify n 0 [] := rfl
 
-instance bitvec.reify_1 {n} : @bitvec.reify n 1 [tt] :=
+instance reify_1 {n} : @reify n 1 [tt] :=
 by cases n; exact rfl
 
-instance bitvec.reify_bit0 {n} (v l) [h : @bitvec.reify n v l] :
-  bitvec.reify (bit0 v) (ff :: l) :=
-bitvec.reify_iff.2 $
-by have := bitvec.of_nat_bit0 n (bitvec.bits_to_nat l);
-   rwa [bitvec.reify_iff.1 h] at this
+instance reify_bit0 {n} (v l) [h : @reify n v l] :
+  reify (bit0 v) (ff :: l) :=
+reify_iff.2 $
+by have := of_nat_bit0 n (bits_to_nat l);
+   rwa [reify_iff.1 h] at this
 
-instance bitvec.reify_bit1 {n} (v l) [h : @bitvec.reify n v l] :
-  bitvec.reify (bit1 v) (tt :: l) :=
-bitvec.reify_iff.2 $
-by have := bitvec.of_nat_bit1 n (bitvec.bits_to_nat l);
-   rwa [bitvec.reify_iff.1 h] at this
+instance reify_bit1 {n} (v l) [h : @reify n v l] :
+  reify (bit1 v) (tt :: l) :=
+reify_iff.2 $
+by have := of_nat_bit1 n (bits_to_nat l);
+   rwa [reify_iff.1 h] at this
+
+theorem bits_to_nat_inj : ∀ {l₁ l₂},
+  bits_to_nat l₁ = bits_to_nat l₂ → l₁.length = l₂.length → l₁ = l₂
+| [] [] _ _ := rfl
+| (a :: l₁) (b :: l₂) e e' := begin
+  rw [bits_to_nat_cons, bits_to_nat_cons] at e,
+  rw [← nat.bodd_bit a (bits_to_nat l₁), e, nat.bodd_bit,
+    @bits_to_nat_inj l₁ l₂ _ (nat.succ_inj e')],
+  rw [← nat.div2_bit a (bits_to_nat l₁), e, nat.div2_bit]
+end
+
+theorem to_nat_inj {n v₁ v₂}
+  (h : @bitvec.to_nat n v₁ = bitvec.to_nat v₂) : v₁ = v₂ :=
+subtype.eq $ bits_to_nat_inj h (v₁.2.trans v₂.2.symm)
+
+end bitvec
+
+namespace x86
+
+def decoder := state_t (list byte) option
+instance : monad decoder := state_t.monad
+
+def read1 : decoder byte :=
+⟨λ l, list.cases_on l none (λ b l, some (b, l))⟩
 
 def split_bits_spec : list (Σ n, bitvec n) → list bool → Prop
 | [] l := list.all l bnot
@@ -185,6 +213,27 @@ begin
         refine ⟨_, h'⟩, simp [vector.cons], exact (nat.bodd_bit _ _).symm } } }
 end
 
+theorem split_bits.determ_l {n₁ n₂ l} (h₁ : split_bits n₁ l) (h₂ : split_bits n₂ l) : n₁ = n₂ :=
+begin
+  induction l generalizing n₁ n₂, {cases h₁, cases h₂, refl},
+  rcases l_hd with ⟨_, l', rfl⟩,
+  induction l' generalizing n₁ n₂,
+  { cases h₁, cases h₂, exact l_ih h₁_a h₂_a },
+  { have : ∀ {n l'},
+      split_bits n l' →
+      l' = ⟨_, l'_hd :: l'_tl, rfl⟩ :: l_tl →
+      l'_hd = nat.bodd n ∧
+      split_bits (nat.div2 n) (⟨_, l'_tl, rfl⟩ :: l_tl),
+    { intros, cases a; try {cases a_1},
+      rcases a_bs with ⟨l₂, rfl⟩,
+      injection a_1, cases h_2,
+      cases congr_arg (λ v : Σ n, bitvec n, v.2.1) h_1,
+      exact ⟨rfl, a_a⟩ },
+    rcases this h₁ rfl with ⟨rfl, h₁'⟩,
+    rcases this h₂ rfl with ⟨e, h₂'⟩,
+    rw [← nat.bit_decomp n₁, e, l'_ih h₁' h₂', nat.bit_decomp] }
+end
+
 theorem split_bits.determ {n l₁ l₂} (h₁ : split_bits n l₁) (h₂ : split_bits n l₂)
   (h : l₁.map sigma.fst = l₂.map sigma.fst) : l₁ = l₂ :=
 begin
@@ -195,26 +244,801 @@ begin
   { cases h₁, cases h₂, cases i_ih _ _ h₁_a h₂_a, refl }
 end
 
+theorem bits_to_byte.determ {n m w1 w2 l} :
+  @bits_to_byte n m w1 l → @bits_to_byte n m w2 l → w1 = w2
+| ⟨e₁, h₁⟩ ⟨_, h₂⟩ := bitvec.to_nat_inj $ split_bits.determ_l h₁ h₂
+
+theorem bits_to_byte.determ_aux {n m w1 w2 l l'} :
+  @bits_to_byte n m w1 l → @bits_to_byte n m w2 (l ++ l') → (w1, l') = (w2, [])
+| ⟨e₁, h₁⟩ ⟨e₂, h₂⟩ := begin
+  simp, suffices, refine ⟨_, this⟩, swap,
+  { apply list.length_eq_zero.1,
+    apply @eq_of_add_eq_add_left _ _ l.length,
+    rw [add_zero, ← list.length_append, e₁, e₂] },
+  clear bits_to_byte.determ_aux, subst this,
+  rw list.append_nil at h₂,
+  exact bitvec.to_nat_inj (split_bits.determ_l h₁ h₂)
+end
+
 theorem read_prefixes.determ {r₁ r₂ l} : read_prefixes r₁ l → read_prefixes r₂ l → r₁ = r₂ :=
 begin
   intros h₁ h₂, cases h₁; cases h₂; congr,
   cases split_bits.determ h₁_a h₂_a rfl, refl,
 end
 
-theorem decode_aux_nil {rex a} : ¬ decode_aux rex a [] :=
-by rintro ⟨⟩; cases e
-
-theorem decode_nil {a} : ¬ decode a [] :=
-begin
-  generalize e : [] = l, rintro ⟨⟩,
-  cases a_1_l1; cases e,
-  exact decode_aux_nil a_1_a_2
-end
-
 @[elab_as_eliminator] theorem byte_split {C : byte → Sort*}
    : ∀ b : byte, (∀ b0 b1 b2 b3 b4 b5 b6 b7,
     C ⟨[b0, b1, b2, b3, b4, b5, b6, b7], rfl⟩) → C b
 | ⟨[b0, b1, b2, b3, b4, b5, b6, b7], rfl⟩ H := H _ _ _ _ _ _ _ _
+
+def binop.from_bits : ∀ (b0 b1 b2 b3 : bool), binop
+| ff ff ff ff := binop.add
+| tt ff ff ff := binop.or
+| ff tt ff ff := binop.adc
+| tt tt ff ff := binop.sbb
+| ff ff tt ff := binop.and
+| tt ff tt ff := binop.sub
+| ff tt tt ff := binop.xor
+| tt tt tt ff := binop.cmp
+| ff ff ff tt := binop.rol
+| tt ff ff tt := binop.ror
+| ff tt ff tt := binop.rcl
+| tt tt ff tt := binop.rcr
+| ff ff tt tt := binop.shl
+| tt ff tt tt := binop.shr
+| ff tt tt tt := binop.tst
+| tt tt tt tt := binop.sar
+
+theorem binop.bits_eq {b0 b1 b2 b3 e op} :
+  binop.bits op ⟨[b0, b1, b2, b3], e⟩ → op = binop.from_bits b0 b1 b2 b3 :=
+begin
+  generalize e' : (⟨[b0, b1, b2, b3], e⟩ : bitvec 4) = v,
+  intro h, induction h;
+  { cases bitvec.reify_eq (congr_arg subtype.val e'), refl }
+end
+
+theorem binop.bits.determ : ∀ {op1 op2 v},
+  binop.bits op1 v → binop.bits op2 v → op1 = op2
+| op1 op2 ⟨[b0, b1, b2, b3], _⟩ h1 h2 :=
+  (binop.bits_eq h1).trans (binop.bits_eq h2).symm
+
+def basic_cond.from_bits : ∀ (b0 b1 b2 : bool), option basic_cond
+| ff ff ff := some basic_cond.o
+| tt ff ff := some basic_cond.b
+| ff tt ff := some basic_cond.e
+| tt tt ff := some basic_cond.na
+| ff ff tt := some basic_cond.s
+| tt ff tt := none
+| ff tt tt := some basic_cond.l
+| tt tt tt := some basic_cond.ng
+
+theorem basic_cond.bits_eq {b0 b1 b2 e c} :
+  basic_cond.bits c ⟨[b0, b1, b2], e⟩ → basic_cond.from_bits b0 b1 b2 = some c :=
+begin
+  generalize e' : (⟨[b0, b1, b2], e⟩ : bitvec 3) = v,
+  intro h, induction h;
+  { cases bitvec.reify_eq (congr_arg subtype.val e'), refl }
+end
+
+def cond_code.from_bits (b0 b1 b2 b3 : bool) : option cond_code :=
+option.map (cond_code.mk b3) (basic_cond.from_bits b0 b1 b2)
+
+theorem cond_code.bits_eq {b0 b1 b2 b3 e c} :
+  cond_code.bits c ⟨[b0, b1, b2, b3], e⟩ → cond_code.from_bits b0 b1 b2 b3 = some c :=
+begin
+  rintro ⟨⟩,
+  rcases split_bits_ok a_a with ⟨h₁, ⟨⟩, _⟩,
+  cases subtype.eq h₁,
+  rw [cond_code.from_bits, basic_cond.bits_eq a_a_1], refl
+end
+
+theorem cond_code.bits.determ : ∀ {c1 c2 v},
+  cond_code.bits c1 v → cond_code.bits c2 v → c1 = c2
+| c1 c2 ⟨[b0, b1, b2, b3], _⟩ h1 h2 := option.some_inj.1 $
+  (cond_code.bits_eq h1).symm.trans (cond_code.bits_eq h2)
+
+theorem read_displacement_ne_3 {mod disp l} :
+  read_displacement mod disp l → mod ≠ 3 :=
+by rintro ⟨⟩ ⟨⟩
+
+theorem read_displacement.determ_aux {mod disp1 disp2 l l'}
+  (h₁ : read_displacement mod disp1 l)
+  (h₂ : read_displacement mod disp2 (l ++ l')) : (disp1, l') = (disp2, []) :=
+begin
+  cases h₁; cases h₂; try {refl},
+  cases bits_to_byte.determ_aux h₁_a h₂_a, refl
+end
+
+theorem read_displacement.determ {mod disp1 disp2 l}
+  (h₁ : read_displacement mod disp1 l)
+  (h₂ : read_displacement mod disp2 l) : disp1 = disp2 :=
+by cases read_displacement.determ_aux h₁
+  (by rw list.append_nil; exact h₂); refl
+
+theorem read_sib_displacement_ne_3 {mod bbase w Base l} :
+  read_sib_displacement mod bbase w Base l → mod ≠ 3 :=
+by rw [read_sib_displacement]; split_ifs; [
+  {rcases h with ⟨_, rfl⟩; rintro _ ⟨⟩},
+  exact λ h, read_displacement_ne_3 h.1]
+
+theorem read_sib_displacement.determ_aux {mod bbase w1 w2 Base1 Base2 l l'}
+  (h₁ : read_sib_displacement mod bbase w1 Base1 l)
+  (h₂ : read_sib_displacement mod bbase w2 Base2 (l ++ l')) : (w1, Base1, l') = (w2, Base2, []) :=
+begin
+  rw read_sib_displacement at h₁ h₂, split_ifs at h₁ h₂,
+  { rcases h₁ with ⟨b, rfl, rfl, rfl⟩,
+    rcases h₂ with ⟨_, rfl, rfl, ⟨⟩⟩, refl },
+  { rcases h₁ with ⟨h1, rfl⟩,
+    rcases h₂ with ⟨h2, rfl⟩,
+    cases read_displacement.determ_aux h1 h2, refl },
+end
+
+theorem read_sib_displacement.determ {mod bbase w1 w2 Base1 Base2 l}
+  (h₁ : read_sib_displacement mod bbase w1 Base1 l)
+  (h₂ : read_sib_displacement mod bbase w2 Base2 l) : (w1, Base1) = (w2, Base2) :=
+by cases read_sib_displacement.determ_aux h₁
+  (by rw list.append_nil; exact h₂); refl
+
+theorem read_SIB_ne_3 {rex mod rm l} :
+  read_SIB rex mod rm l → mod ≠ 3 :=
+by rintro ⟨⟩; exact read_sib_displacement_ne_3 a_a_1
+
+theorem read_SIB.determ_aux {rex mod rm1 rm2 l l'}
+  (h₁ : read_SIB rex mod rm1 l)
+  (h₂ : read_SIB rex mod rm2 (l ++ l')) : (rm1, l') = (rm2, []) :=
+begin
+  cases h₁, cases h₂,
+  cases split_bits.determ h₁_a h₂_a rfl,
+  cases read_sib_displacement.determ_aux h₁_a_1 h₂_a_1, refl
+end
+
+theorem read_SIB.determ {rex mod rm1 rm2 l}
+  (h₁ : read_SIB rex mod rm1 l)
+  (h₂ : read_SIB rex mod rm2 l) : rm1 = rm2 :=
+by cases read_SIB.determ_aux h₁
+  (by rw list.append_nil; exact h₂); refl
+
+theorem read_ModRM_nil {rex reg r} : ¬ read_ModRM rex reg r [] :=
+by rintro ⟨⟩
+
+def read_ModRM' (rex : REX) (r : RM)
+  (rm : bitvec 3) (mod : bitvec 2) (l : list byte) : Prop :=
+if mod = 3 then
+  r = RM.reg (rex_reg rex.B rm) ∧
+  l = []
+else if rm = 4 then
+  read_SIB rex mod r l
+else if rm = 5 ∧ mod = 0 then ∃ i : word,
+  i.to_list_byte l ∧
+  r = RM.mem none base.rip (EXTS i)
+else ∃ disp,
+  read_displacement mod disp l ∧
+  r = RM.mem none (base.reg (rex_reg rex.B rm)) disp
+
+theorem read_ModRM_ModRM' {rex : REX} {reg : regnum} {r : RM}
+  {rm reg_opc : bitvec 3} {mod : bitvec 2} {b : byte} {l : list byte}
+  (h₁ : split_bits b.to_nat [⟨3, rm⟩, ⟨3, reg_opc⟩, ⟨2, mod⟩])
+  (h₂ : read_ModRM rex reg r (b :: l)) :
+  reg = rex_reg rex.R reg_opc ∧ read_ModRM' rex r rm mod l :=
+begin
+  generalize_hyp e : b :: l = l' at h₂,
+  induction h₂; cases e;
+    cases split_bits.determ h₁ h₂_a rfl;
+    refine ⟨rfl, _⟩,
+  { rw [read_ModRM', if_neg, if_neg, if_pos],
+    exact ⟨_, h₂_a_1, rfl⟩,
+    all_goals {exact dec_trivial} },
+  { rw [read_ModRM', if_pos],
+    exact ⟨rfl, rfl⟩, exact dec_trivial },
+  { rw [read_ModRM', if_neg (read_SIB_ne_3 h₂_a_1), if_pos],
+    exact h₂_a_1, refl },
+  { rw [read_ModRM', if_neg (read_displacement_ne_3 h₂_a_3),
+      if_neg h₂_a_1, if_neg h₂_a_2],
+    exact ⟨_, h₂_a_3, rfl⟩ },
+end
+
+theorem read_ModRM_split {rex reg r b l}
+  (h : read_ModRM rex reg r (b :: l)) :
+  ∃ rm reg_opc mod,
+  split_bits b.to_nat [⟨3, rm⟩, ⟨3, reg_opc⟩, ⟨2, mod⟩] :=
+by cases h; exact ⟨_, _, _, by assumption⟩
+
+theorem read_ModRM.determ_aux {rex reg1 r1 reg2 r2 l l'}
+  (h₁ : read_ModRM rex reg1 r1 l)
+  (h₂ : read_ModRM rex reg2 r2 (l ++ l')) :
+  (reg1, r1, l') = (reg2, r2, []) :=
+begin
+  simp,
+  cases l with b l, {cases read_ModRM_nil h₁},
+  rcases read_ModRM_split h₁ with ⟨rm, reg_opc, r, s⟩,
+  rcases read_ModRM_ModRM' s h₁ with ⟨rfl, h₁'⟩,
+  rcases read_ModRM_ModRM' s h₂ with ⟨rfl, h₂'⟩,
+  refine ⟨rfl, _⟩,
+  clear h₁ h₂ s, unfold read_ModRM' at h₁' h₂',
+  split_ifs at h₁' h₂',
+  { rw h₁'.2 at h₂', exact ⟨h₁'.1.trans h₂'.1.symm, h₂'.2⟩ },
+  { cases read_SIB.determ_aux h₁' h₂', exact ⟨rfl, rfl⟩ },
+  { rcases h₁' with ⟨i1, h11, h12⟩,
+    rcases h₂' with ⟨i2, h21, h22⟩,
+    cases bits_to_byte.determ_aux h11 h21,
+    exact ⟨h12.trans h22.symm, rfl⟩ },
+  { rcases h₁' with ⟨i1, h11, h12⟩,
+    rcases h₂' with ⟨i2, h21, h22⟩,
+    cases read_displacement.determ_aux h11 h21,
+    exact ⟨h12.trans h22.symm, rfl⟩ },
+end
+
+theorem read_ModRM.determ {rex reg1 r1 reg2 r2 l}
+  (h₁ : read_ModRM rex reg1 r1 l)
+  (h₂ : read_ModRM rex reg2 r2 l) : (reg1, r1) = (reg2, r2) :=
+by cases read_ModRM.determ_aux h₁
+  (by rw list.append_nil; exact h₂); refl
+
+theorem read_ModRM.determ₂_aux {rex reg1 r1 reg2 r2 l1 l2 l1' l2'}
+  (h₁ : read_ModRM rex reg1 r1 l1)
+  (h₂ : read_ModRM rex reg2 r2 l2)
+  (e : ∃ a', l2 = l1 ++ a' ∧ l1' = a' ++ l2') :
+  (l1, l1') = (l2, l2') :=
+begin
+  rcases e with ⟨l3, rfl, rfl⟩,
+  cases read_ModRM.determ_aux h₁ h₂, simp,
+end
+
+theorem read_ModRM.determ₂ {rex reg1 r1 reg2 r2 l1 l2 l1' l2'}
+  (h₁ : read_ModRM rex reg1 r1 l1)
+  (h₂ : read_ModRM rex reg2 r2 l2)
+  (e : l1 ++ l1' = l2 ++ l2') : (reg1, r1, l1, l1') = (reg2, r2, l2, l2') :=
+begin
+  cases (list.append_eq_append_iff.1 e).elim
+    (λ h, read_ModRM.determ₂_aux h₁ h₂ h)
+    (λ h, (read_ModRM.determ₂_aux h₂ h₁ h).symm),
+  cases read_ModRM.determ h₁ h₂, refl,
+end
+
+theorem read_opcode_ModRM.determ {rex v1 r1 v2 r2 l}
+  (h₁ : read_opcode_ModRM rex v1 r1 l)
+  (h₂ : read_opcode_ModRM rex v2 r2 l) : (v1, r1) = (v2, r2) :=
+begin
+  cases h₁, cases h₂,
+  cases read_ModRM.determ h₁_a h₂_a,
+  cases split_bits.determ h₁_a_1 h₂_a_1 rfl, refl,
+end
+
+theorem read_opcode_ModRM.determ₂ {rex v1 r1 v2 r2 l1 l2 l1' l2'}
+  (h₁ : read_opcode_ModRM rex v1 r1 l1)
+  (h₂ : read_opcode_ModRM rex v2 r2 l2)
+  (e : l1 ++ l1' = l2 ++ l2') : (v1, r1, l1, l1') = (v2, r2, l2, l2') :=
+begin
+  cases h₁, cases h₂,
+  cases read_ModRM.determ₂ h₁_a h₂_a e,
+  cases split_bits.determ h₁_a_1 h₂_a_1 rfl, refl,
+end
+
+theorem read_imm8.determ {w1 w2 l}
+  (h₁ : read_imm8 w1 l) (h₂ : read_imm8 w2 l) : w1 = w2 :=
+by cases h₁; cases h₂; refl
+
+theorem read_imm16.determ {w1 w2 l}
+  (h₁ : read_imm16 w1 l) (h₂ : read_imm16 w2 l) : w1 = w2 :=
+by cases h₁; cases h₂; cases bits_to_byte.determ h₁_a h₂_a; refl
+
+theorem read_imm32.determ {w1 w2 l}
+  (h₁ : read_imm32 w1 l) (h₂ : read_imm32 w2 l) : w1 = w2 :=
+by cases h₁; cases h₂; cases bits_to_byte.determ h₁_a h₂_a; refl
+
+theorem read_imm.determ : ∀ {sz w1 w2 l},
+  read_imm sz w1 l → read_imm sz w2 l → w1 = w2
+| (wsize.Sz8 _) _ _ _ := read_imm8.determ
+| wsize.Sz16 _ _ _ := read_imm16.determ
+| wsize.Sz32 _ _ _ := read_imm32.determ
+| wsize.Sz64 _ _ _ := false.elim
+
+theorem read_full_imm.determ : ∀ {sz w1 w2 l},
+  read_full_imm sz w1 l → read_full_imm sz w2 l → w1 = w2
+| (wsize.Sz8 _) _ _ _ := read_imm8.determ
+| wsize.Sz16 _ _ _ := read_imm16.determ
+| wsize.Sz32 _ _ _ := read_imm32.determ
+| wsize.Sz64 _ _ _ := bits_to_byte.determ
+
+def decode_two' (rex : REX) (a : ast) (b0 b1 b2 b3 b4 b5 b6 b7 : bool) (l : list byte) : Prop :=
+cond b7
+  (cond b6
+    ( -- xadd
+      [b1, b2, b3, b4, b5] = [ff, ff, ff, ff, ff] ∧
+      let v := b0, sz := op_size_W rex v in
+      ∃ reg r,
+      read_ModRM rex reg r l ∧
+      a = ast.xadd sz r reg)
+    (cond b5
+      (cond b2
+        ( -- movsx
+          [b1, b4] = [tt, tt] ∧
+          let sz2 := op_size_W rex tt,
+              sz := if b0 then wsize.Sz16 else wsize.Sz8 rex.is_some in
+          ∃ reg r,
+          read_ModRM rex reg r l ∧
+          a = (if b3 then ast.movsx else ast.movzx) sz (dest_src.R_rm reg r) sz2)
+        ( -- cmpxchg
+          [b1, b4] = [ff, tt] ∧
+          let v := b0, sz := op_size_W rex v in
+          ∃ reg r,
+          read_ModRM rex reg r l ∧
+          a = ast.cmpxchg sz r reg))
+      (cond b4
+        ( -- setcc
+          ∃ reg r code,
+          read_ModRM rex reg r l ∧
+          cond_code.from_bits b0 b1 b2 b3 = some code ∧
+          a = ast.setcc code rex.is_some r)
+        ( -- jcc
+          ∃ imm code,
+          read_imm32 imm l ∧
+          cond_code.from_bits b0 b1 b2 b3 = some code ∧
+          a = ast.jcc code imm))))
+  (cond b6
+    ( -- cmov
+      [b4, b5] = [ff, ff] ∧
+      let sz := op_size tt rex.W tt in
+      ∃ reg r code,
+      read_ModRM rex reg r l ∧
+      cond_code.from_bits b0 b1 b2 b3 = some code ∧
+      a = ast.cmov code sz (dest_src.R_rm reg r))
+    ( -- syscall
+      [b0, b1, b2, b3, b4, b5] = [tt, ff, tt, ff, ff, ff] ∧
+      a = ast.syscall ∧
+      l = []))
+
+theorem decode_two_two' {rex a b0 b1 b2 b3 b4 b5 b6 b7 l} :
+  decode_two rex a (⟨[b0, b1, b2, b3, b4, b5, b6, b7], rfl⟩ :: l) →
+  decode_two' rex a b0 b1 b2 b3 b4 b5 b6 b7 l :=
+begin
+  generalize e : (⟨[b0, b1, b2, b3, b4, b5, b6, b7], rfl⟩ :: l : list byte) = l',
+  intro a, cases a,
+  { cases e, rcases split_bits_ok a_a with ⟨h₁, h₂, _⟩,
+    cases subtype.eq h₁,
+    cases bitvec.reify_eq h₂,
+    exact ⟨rfl, _, _, _, a_a_1, cond_code.bits_eq a_a_2, rfl⟩ },
+  { cases e, rcases split_bits_ok a_a with ⟨h₁, h₂, _⟩,
+    cases subtype.eq h₁,
+    cases bitvec.reify_eq h₂,
+    exact ⟨_, _, a_a_1, cond_code.bits_eq a_a_2, rfl⟩ },
+  { cases e, rcases split_bits_ok a_a with ⟨h₁, h₂, _⟩,
+    cases subtype.eq h₁,
+    cases bitvec.reify_eq h₂,
+    exact ⟨_, _, _, a_a_1, cond_code.bits_eq a_a_2, rfl⟩ },
+  { cases e, rcases split_bits_ok a_a with ⟨⟨⟩, h₁, _⟩,
+    cases bitvec.reify_eq h₁,
+    exact ⟨rfl, _, _, a_a_1, rfl⟩ },
+  { cases e, rcases split_bits_ok a_a with ⟨⟨⟩, h₁, ⟨⟩, h₂, _⟩,
+    cases bitvec.reify_eq h₁,
+    cases bitvec.reify_eq h₂,
+    exact ⟨rfl, _, _, a_a_1, rfl⟩ },
+  { cases e, rcases split_bits_ok a_a with ⟨⟨⟩, h₁, _⟩,
+    cases bitvec.reify_eq h₁,
+    exact ⟨rfl, _, _, a_a_1, rfl⟩ },
+  { injection e, cases congr_arg subtype.val (bitvec.reify_eq' h_1),
+    cases h_2, exact ⟨rfl, rfl, rfl⟩ },
+end
+
+theorem decode_two_nil {rex a} : ¬ decode_two rex a [].
+
+theorem decode_two.determ {rex a₁ a₂ l} : decode_two rex a₁ l → decode_two rex a₂ l → a₁ = a₂ :=
+begin
+  cases l with b l, {exact decode_two_nil.elim},
+  apply byte_split b, introv h1 h2,
+  replace h1 := decode_two_two' h1,
+  replace h2 := decode_two_two' h2,
+  unfold decode_two' at h1 h2,
+  repeat { do
+    `(cond %%e _ _) ← tactic.get_local `h1 >>= tactic.infer_type,
+    tactic.cases e $> (); `[dsimp only [cond] at h1 h2] },
+  { exact h1.2.1.trans h2.2.1.symm },
+  { rcases h1.2 with ⟨reg1, r1, h11, h12, h13, rfl⟩,
+    rcases h2.2 with ⟨reg2, r2, h21, h22, h23, rfl⟩,
+    cases read_ModRM.determ h12 h22,
+    cases h13.symm.trans h23, refl },
+  { rcases h1 with ⟨imm1, code1, h11, h12, rfl⟩,
+    rcases h2 with ⟨imm2, code2, h21, h22, rfl⟩,
+    cases read_imm32.determ h11 h21,
+    cases h12.symm.trans h22, refl },
+  { rcases h1 with ⟨reg1, r1, code1, h11, h12, rfl⟩,
+    rcases h2 with ⟨reg2, r2, code2, h21, h22, rfl⟩,
+    cases read_ModRM.determ h11 h21,
+    cases h12.symm.trans h22, refl },
+  { rcases h1 with ⟨reg1, r1, code1, h11, h12, rfl⟩,
+    rcases h2 with ⟨reg2, r2, code2, h21, h22, rfl⟩,
+    cases read_ModRM.determ h11 h21, refl },
+  { rcases h1.2 with ⟨reg1, r1, h11, rfl⟩,
+    rcases h2.2 with ⟨reg2, r2, h21, rfl⟩,
+    cases read_ModRM.determ h11 h21, refl },
+  { rcases h1.2 with ⟨reg1, r1, h11, rfl⟩,
+    rcases h2.2 with ⟨reg2, r2, h21, rfl⟩,
+    cases read_ModRM.determ h11 h21, refl },
+end
+
+def decode_hi' (v : bool) (sz : wsize) (r : RM) :
+  ∀ (b0 b1 b2 x : bool), ast → list byte → Prop
+| ff ff ff ff a l := ∃ imm,
+                      read_imm sz imm l ∧
+                      a = ast.binop binop.tst sz (dest_src.Rm_i r imm)
+| ff tt ff ff a l := a = ast.unop unop.not sz r ∧ l = []
+| tt tt ff ff a l := a = ast.unop unop.neg sz r ∧ l = []
+| ff ff tt ff a l := a = ast.mul sz r ∧ l = []
+| ff tt tt ff a l := a = ast.div sz r ∧ l = []
+| ff ff ff tt a l := a = ast.unop unop.inc sz r ∧ l = []
+| tt ff ff tt a l := a = ast.unop unop.dec sz r ∧ l = []
+| ff tt ff tt a l := a = ast.call (imm_rm.rm r) ∧ l = []
+| ff ff tt tt a l := a = ast.jump r ∧ l = []
+| ff tt tt tt a l := a = ast.push (imm_rm.rm r) ∧ l = []
+| _  _  _  _  a l := false
+
+theorem decode_hi_hi' {v sz r x b0 b1 b2 a l}
+  (h : decode_hi v sz r x ⟨[b0, b1, b2], rfl⟩ a l) : decode_hi' v sz r b0 b1 b2 x a l :=
+begin
+  generalize_hyp e : (⟨[b0, b1, b2], rfl⟩ : bitvec 3) = opc at h,
+  induction h; cases congr_arg subtype.val (bitvec.reify_eq' e),
+  exact ⟨_, h_a, rfl⟩, all_goals { exact ⟨rfl, rfl⟩ }
+end
+
+theorem decode_hi.determ {v sz r x a1 a2 l} : ∀ {opc},
+  decode_hi v sz r x opc a1 l → decode_hi v sz r x opc a2 l → a1 = a2
+| ⟨[b0, b1, b2], _⟩ h1 h2 := begin
+  replace h1 := decode_hi_hi' h1,
+  replace h2 := decode_hi_hi' h2, clear decode_hi.determ,
+  cases b0; cases b1; cases b2; cases x; cases h1; cases h2,
+  { cases read_imm.determ h1_h.1 h2_h.1,
+    exact h1_h.2.trans h2_h.2.symm },
+  all_goals { exact h1_left.trans h2_left.symm }
+end
+
+def decode_aux' (rex : REX) (a : ast) (b0 b1 b2 b3 b4 b5 b6 b7 : bool) (l : list byte) : Prop :=
+cond b7
+  (cond b6
+    (cond b5
+      (cond b4
+        (cond b2
+          (cond b1
+            ( -- hi
+              let v := b0, sz := op_size_W rex v in
+              ∃ opc r l1 l2,
+              read_opcode_ModRM rex opc r l1 ∧
+              decode_hi v sz r b3 opc a l2 ∧
+              l = l1 ++ l2)
+            ( -- cmc
+              b0 = tt ∧
+              a = ast.cmc ∧
+              l = []))
+          ( -- clc, stc
+            [b1, b3] = [ff, tt] ∧
+            a = cond b0 ast.stc ast.clc ∧
+            l = []))
+        (cond b0
+          ( -- jump
+            [b2, b3] = [ff, tt] ∧
+            ∃ imm,
+            (if b1 then read_imm8 imm l else read_imm32 imm l) ∧
+            a = ast.jcc cond_code.always imm)
+          ( -- call
+           [b2, b3] = [ff, tt] ∧
+            ∃ imm,
+            read_imm32 imm l ∧
+            a = ast.call (imm_rm.imm imm))))
+      ( let v := b0, sz := op_size_W rex v in
+        cond b4
+        ( -- binop_hi_reg
+          [b2, b3] = [ff, ff] ∧
+          ∃ opc r op,
+          read_opcode_ModRM rex opc r l ∧ opc ≠ 6 ∧
+          binop.bits op (rex_reg tt opc) ∧
+          let src_dst := if b1 then dest_src.Rm_r r RCX else dest_src.Rm_i r 1 in
+          a = ast.binop op sz src_dst)
+        (cond b3
+          ( -- leave
+            [b0, b1, b2] = [tt, ff, ff] ∧
+            a = ast.leave ∧
+            l = [])
+          (cond b2
+            ( -- mov_imm
+              b1 = tt ∧
+              ∃ opc r imm l1 l2,
+              read_opcode_ModRM rex opc r l1 ∧
+              read_imm sz imm l2 ∧
+              a = ast.mov sz (dest_src.Rm_i r imm) ∧
+              l = l1 ++ l2)
+            (cond b1
+              ( -- ret
+                ∃ imm,
+                (if v then imm = 0 ∧ l = [] else read_imm16 imm l) ∧
+                a = ast.ret imm)
+              ( -- binop_hi
+                ∃ opc r imm op l1 l2,
+                read_opcode_ModRM rex opc r l1 ∧ opc ≠ 6 ∧
+                binop.bits op (rex_reg tt opc) ∧
+                read_imm8 imm l2 ∧
+                a = ast.binop op sz (dest_src.Rm_i r imm) ∧
+                l = l1 ++ l2))))))
+    (cond b5
+      (cond b4
+        ( -- mov64
+          let v := b3, sz := op_size_W rex v in
+          ∃ imm,
+          read_full_imm sz imm l ∧
+          a = ast.mov sz (dest_src.Rm_i (RM.reg ⟨[b0, b1, b2, rex.B], rfl⟩) imm))
+        ( -- test_rax
+          [b1, b2, b3] = [ff, ff, tt] ∧
+          let v := b0, sz := op_size tt rex.W v in
+          ∃ imm,
+          read_imm sz imm l ∧
+          a = ast.binop binop.tst sz (dest_src.Rm_i (RM.reg RAX) imm)))
+      (cond b4
+        ( -- xchg_rax
+          b3 = ff ∧
+          let sz := op_size tt rex.W tt in
+          a = ast.xchg sz (RM.reg RAX) ⟨[b0, b1, b2, rex.B], rfl⟩ ∧
+          l = [])
+        (cond b3
+          (cond b2
+            (cond b1
+              ( -- pop_rm
+                b0 = tt ∧
+                ∃ r,
+                read_opcode_ModRM rex 0 r l ∧
+                a = ast.pop r)
+              ( -- lea
+                b0 = tt ∧
+                ∃ reg r,
+                let sz := op_size tt rex.W tt in
+                read_ModRM rex reg r l ∧ RM.is_mem r ∧
+                a = ast.lea sz (dest_src.R_rm reg r)))
+            ( -- mov
+              let v := b0, sz := op_size_W rex v in
+              ∃ reg r,
+              read_ModRM rex reg r l ∧
+              let src_dst := if b1 then dest_src.R_rm reg r else dest_src.Rm_r r reg in
+              a = ast.mov sz src_dst))
+          (cond b2
+            ( let v := b0, sz := op_size_W rex v in
+              -- xchg, test
+              ∃ reg r,
+              read_ModRM rex reg r l ∧
+              a = cond b1 (ast.xchg sz r reg)
+                (ast.binop binop.tst sz (dest_src.Rm_r r reg)))
+            ( -- binop_imm, binop_imm8
+              let sz := op_size_W rex (cond b1 tt b0) in
+              ∃ opc r l1 imm l2 op,
+              read_opcode_ModRM rex opc r l1 ∧
+              binop.bits op (EXTZ opc) ∧
+              cond b1 (read_imm8 imm l2) (read_imm sz imm l2) ∧
+              a = ast.binop op sz (dest_src.Rm_i r imm) ∧
+              l = l1 ++ l2))))))
+  (cond b6
+    (cond b5
+      (cond b4
+        ( -- jcc8
+          ∃ code imm,
+          cond_code.from_bits b0 b1 b2 b3 = some code ∧
+          read_imm8 imm l ∧
+          a = ast.jcc code imm)
+        (cond b3
+          ( -- push_imm
+            [b0, b2] = [ff, ff] ∧
+            ∃ imm,
+            read_imm (if b1 then wsize.Sz8 ff else wsize.Sz32) imm l ∧
+            a = ast.push (imm_rm.imm imm))
+          ( -- movsx
+            [b0, b1, b2] = [tt, tt, ff] ∧
+            ∃ reg r,
+            read_ModRM rex reg r l ∧
+            a = ast.movsx wsize.Sz32 (dest_src.R_rm reg r) wsize.Sz64)))
+      ( -- pop, push_rm
+        b4 = tt ∧
+        let reg := RM.reg ⟨[b0, b1, b2, rex.B], rfl⟩ in
+        a = cond b3 (ast.pop reg) (ast.push (imm_rm.rm reg)) ∧
+        l = []))
+    (cond b2
+      (cond b1
+        ( -- decode_two
+          [b0, b3, b4, b5] = [tt, tt, ff, ff] ∧
+          decode_two rex a l)
+        ( -- binop_imm_rax
+          let v := b0, sz := op_size_W rex v,
+              op := binop.from_bits b3 b4 b5 ff in
+          ∃ imm, read_imm sz imm l ∧
+          a = ast.binop op sz (dest_src.Rm_i (RM.reg RAX) imm)))
+      ( -- binop1
+        let v := b0, d := b1, sz := op_size_W rex v,
+            op := binop.from_bits b3 b4 b5 ff in
+        ∃ reg r, read_ModRM rex reg r l ∧
+        let src_dst := if d then dest_src.R_rm reg r else dest_src.Rm_r r reg in
+        a = ast.binop op sz src_dst)))
+
+theorem decode_aux_aux' {rex a b0 b1 b2 b3 b4 b5 b6 b7 l} :
+  decode_aux rex a (⟨[b0, b1, b2, b3, b4, b5, b6, b7], rfl⟩ :: l) →
+  decode_aux' rex a b0 b1 b2 b3 b4 b5 b6 b7 l :=
+begin
+  generalize e : (⟨[b0, b1, b2, b3, b4, b5, b6, b7], rfl⟩ :: l : list byte) = l',
+  intro a, cases a,
+  { cases e, rcases split_bits_ok a_a with ⟨⟨⟩, ⟨⟩, ⟨⟩, h₁, h₂, _⟩,
+    cases subtype.eq h₁,
+    cases bitvec.reify_eq h₂,
+    cases binop.bits_eq a_a_2,
+    exact ⟨_, _, a_a_1, rfl⟩ },
+  { cases e, rcases split_bits_ok a_a with ⟨⟨⟩, h₁, h₂, h₃, _⟩,
+    cases bitvec.reify_eq h₁,
+    cases subtype.eq h₂,
+    cases bitvec.reify_eq h₃,
+    cases binop.bits_eq a_a_1,
+    exact ⟨_, a_a_2, rfl⟩ },
+  { cases e, rcases split_bits_ok a_a with ⟨⟨⟩, h₁, _⟩,
+    cases bitvec.reify_eq h₁,
+    exact ⟨_, _, _, _, _, _, a_a_1, a_a_3, a_a_2, rfl, rfl⟩ },
+  { injection e, cases congr_arg subtype.val (bitvec.reify_eq' h_1),
+    exact ⟨_, _, _, _, _, _, a_a, a_a_1, a_a_2, rfl, h_2⟩ },
+  { cases e, rcases split_bits_ok a_a with ⟨⟨⟩, h₁, _⟩,
+    cases bitvec.reify_eq h₁,
+    exact ⟨_, _, _, _, _, _, a_a_1, a_a_2, a_a_3, a_a_4, rfl, rfl⟩ },
+  { cases e, rcases split_bits_ok a_a with ⟨⟨⟩, ⟨⟩, h₁, _⟩,
+    cases bitvec.reify_eq h₁,
+    exact ⟨rfl, _, _, _, a_a_1, a_a_2, a_a_3, rfl⟩ },
+  { injection e, cases congr_arg subtype.val (bitvec.reify_eq' h_1),
+    cases h_2, exact ⟨rfl, a_a_1⟩ },
+  { injection e, cases congr_arg subtype.val (bitvec.reify_eq' h_1),
+    cases h_2, exact ⟨rfl, _, _, a_a, rfl⟩ },
+  { cases e, rcases split_bits_ok a_a with ⟨⟨⟩, ⟨⟩, h₁, _⟩,
+    cases bitvec.reify_eq h₁,
+    exact ⟨_, _, a_a_1, rfl⟩ },
+  { cases e, rcases split_bits_ok a_a with ⟨h₁, ⟨⟩, h₂, _⟩,
+    cases subtype.eq h₁,
+    cases bitvec.reify_eq h₂,
+    exact ⟨_, a_a_1, rfl⟩ },
+  { cases e, rcases split_bits_ok a_a with ⟨⟨⟩, h₁, _⟩,
+    cases bitvec.reify_eq h₁,
+    exact ⟨rfl, _, _, _, _, _, a_a_1, a_a_2, rfl, rfl⟩ },
+  { cases e, rcases split_bits_ok a_a with ⟨⟨⟩, h₁, _⟩,
+    cases bitvec.reify_eq h₁,
+    exact ⟨_, _, a_a_1, rfl⟩ },
+  { cases e, rcases split_bits_ok a_a with ⟨h₁, h₂, _⟩,
+    cases subtype.eq h₁,
+    cases bitvec.reify_eq h₂,
+    exact ⟨rfl, rfl, rfl⟩ },
+  { cases e, rcases split_bits_ok a_a with ⟨⟨⟩, ⟨⟩, h₁, _⟩,
+    cases bitvec.reify_eq h₁,
+    exact ⟨rfl, _, a_a_1, rfl⟩ },
+  { cases e, rcases split_bits_ok a_a with ⟨h₁, h₂, _⟩,
+    cases subtype.eq h₁,
+    cases bitvec.reify_eq h₂,
+    exact ⟨rfl, rfl, rfl⟩ },
+  { cases e, rcases split_bits_ok a_a with ⟨h₁, h₂, _⟩,
+    cases subtype.eq h₁,
+    cases bitvec.reify_eq h₂,
+    exact ⟨rfl, rfl, rfl⟩ },
+  { injection e, cases congr_arg subtype.val (bitvec.reify_eq' h_1),
+    cases h_2, exact ⟨rfl, _, a_a, rfl⟩ },
+  { cases e, rcases split_bits_ok a_a with ⟨⟨⟩, ⟨⟩, h₁, _⟩,
+    cases bitvec.reify_eq h₁,
+    exact ⟨rfl, _, a_a_1, rfl⟩ },
+  { cases e, rcases split_bits_ok a_a with ⟨h₁, h₂, _⟩,
+    cases subtype.eq h₁,
+    cases bitvec.reify_eq h₂,
+    exact ⟨_, _, cond_code.bits_eq a_a_1, a_a_2, rfl⟩ },
+  { injection e, cases congr_arg subtype.val (bitvec.reify_eq' h_1),
+    cases h_2, exact ⟨rfl, _, a_a, rfl⟩ },
+  { cases e, rcases split_bits_ok a_a with ⟨⟨⟩, h₁, _⟩,
+    cases bitvec.reify_eq h₁,
+    exact ⟨_, a_a_1, rfl⟩ },
+  { injection e, cases congr_arg subtype.val (bitvec.reify_eq' h_1),
+    cases h_2, exact ⟨rfl, rfl, rfl⟩ },
+  { injection e, cases congr_arg subtype.val (bitvec.reify_eq' h_1),
+    cases h_2, exact ⟨rfl, _, _, a_a, a_a_1, rfl⟩ },
+  { cases e, rcases split_bits_ok a_a with ⟨⟨⟩, h₁, _⟩,
+    cases bitvec.reify_eq h₁,
+    exact ⟨_, _, a_a_1, rfl⟩ },
+  { cases e, rcases split_bits_ok a_a with ⟨⟨⟩, h₁, _⟩,
+    cases bitvec.reify_eq h₁,
+    exact ⟨rfl, _, a_a_1, rfl⟩ },
+  { injection e, cases congr_arg subtype.val (bitvec.reify_eq' h_1),
+    cases h_2, exact ⟨rfl, rfl, rfl⟩ },
+  { injection e, cases congr_arg subtype.val (bitvec.reify_eq' h_1),
+    cases h_2, exact ⟨rfl, rfl, rfl⟩ },
+  { injection e, cases congr_arg subtype.val (bitvec.reify_eq' h_1),
+    cases h_2, exact ⟨rfl, rfl, rfl⟩ },
+  { cases e, rcases split_bits_ok a_a_1 with ⟨⟨⟩, h₁, ⟨⟩, h₂, _⟩,
+    cases bitvec.reify_eq h₁,
+    cases bitvec.reify_eq h₂,
+    exact ⟨_, _, _, _, a_a_2, a_a_3, rfl⟩ },
+end
+
+theorem decode_aux_nil {rex a} : ¬ decode_aux rex a [].
+
+theorem decode_aux.determ {rex a₁ a₂ l} : decode_aux rex a₁ l → decode_aux rex a₂ l → a₁ = a₂ :=
+begin
+  cases l with b l, {exact decode_aux_nil.elim},
+  apply byte_split b, introv h1 h2,
+  replace h1 := decode_aux_aux' h1,
+  replace h2 := decode_aux_aux' h2,
+  unfold decode_aux' at h1 h2,
+  repeat { do
+    `(cond %%e _ _) ← tactic.get_local `h1 >>= tactic.infer_type,
+    tactic.cases e $> (); `[dsimp only [cond] at h1 h2] },
+  { rcases h1 with ⟨reg1, r1, h11, rfl⟩,
+    rcases h2 with ⟨reg2, r2, h21, rfl⟩,
+    cases read_ModRM.determ h11 h21, refl },
+  { rcases h1 with ⟨imm1, h11, rfl⟩,
+    rcases h2 with ⟨imm2, h21, rfl⟩,
+    cases read_imm.determ h11 h21, refl },
+  { exact decode_two.determ h1.2 h2.2 },
+  { exact h1.2.1.trans h2.2.1.symm },
+  { rcases h1.2 with ⟨reg1, r1, h11, rfl⟩,
+    rcases h2.2 with ⟨reg2, r2, h21, rfl⟩,
+    cases read_ModRM.determ h11 h21, refl },
+  { rcases h1.2 with ⟨imm1, h11, rfl⟩,
+    rcases h2.2 with ⟨imm2, h21, rfl⟩,
+    cases read_imm.determ h11 h21, refl },
+  { rcases h1 with ⟨code1, imm1, h11, h12, rfl⟩,
+    rcases h2 with ⟨code2, imm2, h21, h22, rfl⟩,
+    cases h11.symm.trans h21,
+    cases read_imm8.determ h12 h22, refl },
+  { rcases h1 with ⟨opc1, r1, l11, imm1, l12, op1, h11, h12, h13, rfl, rfl⟩,
+    rcases h2 with ⟨opc2, r2, l21, imm2, l22, op2, h21, h22, h23, rfl, e⟩,
+    cases read_opcode_ModRM.determ₂ h11 h21 e,
+    cases binop.bits.determ h12 h22,
+    cases b1,
+    { cases read_imm.determ h13 h23, refl },
+    { cases read_imm8.determ h13 h23, refl } },
+  { rcases h1 with ⟨reg1, r1, h11, rfl⟩,
+    rcases h2 with ⟨reg2, r2, h21, rfl⟩,
+    cases read_ModRM.determ h11 h21, refl },
+  { rcases h1 with ⟨reg1, r1, h11, rfl⟩,
+    rcases h2 with ⟨reg2, r2, h21, rfl⟩,
+    cases read_ModRM.determ h11 h21, refl },
+  { rcases h1.2 with ⟨reg1, r1, h11, h12, rfl⟩,
+    rcases h2.2 with ⟨reg2, r2, h21, h22, rfl⟩,
+    cases read_ModRM.determ h11 h21, refl },
+  { rcases h1.2 with ⟨r1, h11, h12, rfl⟩,
+    rcases h2.2 with ⟨r2, h21, h22, rfl⟩,
+    cases read_opcode_ModRM.determ h11 h21, refl },
+  { rcases h1.2 with rfl,
+    rcases h2.2 with rfl, refl },
+  { rcases h1.2 with ⟨imm1, h11, rfl⟩,
+    rcases h2.2 with ⟨imm2, h21, rfl⟩,
+    cases read_imm.determ h11 h21, refl },
+  { rcases h1 with ⟨imm1, h11, rfl⟩,
+    rcases h2 with ⟨imm2, h21, rfl⟩,
+    cases read_full_imm.determ h11 h21, refl },
+  { rcases h1 with ⟨opc1, r1, imm1, op1, l11, l12, h11, _, h12, h13, rfl, rfl⟩,
+    rcases h2 with ⟨opc2, r2, imm2, op2, l21, l22, h21, _, h22, h23, rfl, e⟩,
+    cases read_opcode_ModRM.determ₂ h11 h21 e,
+    cases binop.bits.determ h12 h22,
+    cases read_imm8.determ h13 h23, refl },
+  { rcases h1 with ⟨imm1, h11, rfl⟩,
+    rcases h2 with ⟨imm2, h21, rfl⟩,
+    split_ifs at h11 h21,
+    { cases h11.1.trans h21.1.symm, refl },
+    { cases read_imm16.determ h11 h21, refl } },
+  { rcases h1 with ⟨opc1, r1, imm1, op1, l11, l12, h11, h12, rfl, rfl⟩,
+    rcases h2 with ⟨opc2, r2, imm2, op2, l21, l22, h21, h22, rfl, e⟩,
+    cases read_opcode_ModRM.determ₂ h11 h21 e,
+    cases read_imm.determ h12 h22, refl },
+  { exact h1.2.1.trans h2.2.1.symm },
+  { rcases h1.2 with ⟨opc1, r1, op1, h11, _, h12, rfl⟩,
+    rcases h2.2 with ⟨opc2, r2, op2, h21, _, h22, rfl⟩,
+    cases read_opcode_ModRM.determ h11 h21,
+    cases binop.bits.determ h12 h22, refl },
+  { rcases h1.2 with ⟨imm1, h11, rfl⟩,
+    rcases h2.2 with ⟨imm2, h21, rfl⟩,
+    cases read_imm32.determ h11 h21, refl },
+  { rcases h1.2 with ⟨imm1, h11, rfl⟩,
+    rcases h2.2 with ⟨imm2, h21, rfl⟩,
+    split_ifs at h11 h21,
+    { cases read_imm8.determ h11 h21, refl },
+    { cases read_imm32.determ h11 h21, refl } },
+  { exact h1.2.1.trans h2.2.1.symm },
+  { exact h1.2.1.trans h2.2.1.symm },
+  { rcases h1 with ⟨opc1, r1, l11, l12, h11, h12, rfl⟩,
+    rcases h2 with ⟨opc2, r2, l21, l22, h21, h22, e⟩,
+    cases read_opcode_ModRM.determ₂ h11 h21 e,
+    exact decode_hi.determ h12 h22 },
+end
 
 theorem decode.no_prefix {rex rex' a l b l'} :
   read_prefixes rex l → b ∈ l → ¬ decode_aux rex' a (b :: l') :=
@@ -255,8 +1079,12 @@ begin
   { cases e, rcases split_bits_ok a_2_a_1 with ⟨_, _, _, h, _⟩, cases bitvec.reify_eq h },
 end
 
-theorem decode_aux.determ {rex a₁ a₂ l} : decode_aux rex a₁ l → decode_aux rex a₂ l → a₁ = a₂ :=
-sorry
+theorem decode_nil {a} : ¬ decode a [] :=
+begin
+  generalize e : [] = l, rintro ⟨⟩,
+  cases a_1_l1; cases e,
+  exact decode_aux_nil a_1_a_2
+end
 
 theorem decode.determ : ∀ {a₁ a₂ l}, decode a₁ l → decode a₂ l → a₁ = a₂ :=
 suffices ∀ {a₁ a₂ : ast}
